@prefix rdf: <http://www.w3.org/1999/02/22-rdf-syntax-ns#> .

<http://eccenca.com/mobivoc/Ampere>
    a rdf:Property, <http://www.w3.org/2002/07/owl#DatatypeProperty> ;
    <http://www.w3.org/2000/01/rdf-schema#comment> "Represents the flow rate of electric charge." ;
    <http://www.w3.org/2000/01/rdf-schema#domain> <http://eccenca.com/mobivoc/Battery> ;
    <http://www.w3.org/2000/01/rdf-schema#label> "Ampere"@de, "Ampere"@en ;
    <http://www.w3.org/2000/01/rdf-schema#range> <http://www.w3.org/2000/01/rdf-schema#Literal> .

<http://eccenca.com/mobivoc/DeepCycle>
    <http://www.w3.org/2000/01/rdf-schema#comment> "A lead-acid battery designed to be regularly deeply discharged using most of its capacity." ;
    <http://www.w3.org/2000/01/rdf-schema#label> "****Batterie"@de, "Deep-Cycle Battery"@en ;
    <http://www.w3.org/2000/01/rdf-schema#subClassOf> <http://eccenca.com/mobivoc/LeadAcid> .

<http://eccenca.com/mobivoc/DieselBatteryHybrid>
    <http://www.w3.org/2000/01/rdf-schema#comment> "*****" ;
    <http://www.w3.org/2000/01/rdf-schema#label> "DieselBatterieHybrid"@de, "DieselBatteryHybrid"@en ;
    <http://www.w3.org/2000/01/rdf-schema#subClassOf> <http://eccenca.com/mobivoc/Battery> .

<http://eccenca.com/mobivoc/ElectricVehicleBattery>
    a <http://www.w3.org/2000/01/rdf-schema#Class>, <http://www.w3.org/2002/07/owl#Class> ;
    <http://www.w3.org/2000/01/rdf-schema#altlabel> "Traction battery"@en, "Traktionsakku"@de ;
    <http://www.w3.org/2000/01/rdf-schema#comment> "A battery used to power the propulsion of a battery electric vehicle." ;
    <http://www.w3.org/2000/01/rdf-schema#label> "Electric Vehicle Battery"@en, "Traktionsbatterie"@de ;
    <http://www.w3.org/2004/02/skos/core#hiddenLabel> "Antriebsbatterie"@de, "EVB"@en .

<http://eccenca.com/mobivoc/FloodedLeadAcid>
    <http://www.w3.org/2000/01/rdf-schema#comment> "Flooded lead acid batteries have cells with liquid electrolyte and are available in flat and tubular plate constructions with a wide variety of plate sizes." ;
    <http://www.w3.org/2000/01/rdf-schema#label> " Blei-Säure-Batterie"@de, "Flooded Lead-Acid Battery"@en ;
    <http://www.w3.org/2000/01/rdf-schema#subClassOf> <http://eccenca.com/mobivoc/LeadAcid> .

<http://eccenca.com/mobivoc/LeadAcid>
    <http://www.w3.org/2000/01/rdf-schema#comment> "The oldest type of rechargeable battery. The cells have a relatively large power-to-weight ratio and these batteries have low cost." ;
    <http://www.w3.org/2000/01/rdf-schema#label> "Bleiakkumulator"@de, "Lead-Acid Battery"@en ;
    <http://www.w3.org/2000/01/rdf-schema#subClassOf> <http://eccenca.com/mobivoc/Battery> .

<http://eccenca.com/mobivoc/LithiumIon>
    <http://www.w3.org/2000/01/rdf-schema#altlabel> "Li-ion battery"@en, "Lithium-Akkumulator"@de ;
    <http://www.w3.org/2000/01/rdf-schema#comment> "One of the most popular types of rechargeable batteries for electric vehicles. They use an intercalated lithium compound as one electrode material." ;
    <http://www.w3.org/2000/01/rdf-schema#label> "Lithium-Ionen-Akkumulator"@de, "Lithium-ion Battery"@en ;
    <http://www.w3.org/2000/01/rdf-schema#subClassOf> <http://eccenca.com/mobivoc/Battery> ;
    <http://www.w3.org/2004/02/skos/core#hiddenLabel> "LIB"@en .

<http://eccenca.com/mobivoc/LithiumIonPolymer>
    <http://www.w3.org/2000/01/rdf-schema#altlabel> "LiPo"@en, "LiPoly"@de ;
    <http://www.w3.org/2000/01/rdf-schema#comment> "A rechargeable battery of lithium-ion technology in a pouch format." ;
    <http://www.w3.org/2000/01/rdf-schema#label> "Lithium Polymer Battery"@en, "Lithium-Polymer-Akkumulator"@de ;
    <http://www.w3.org/2000/01/rdf-schema#subClassOf> <http://eccenca.com/mobivoc/Battery> .

<http://eccenca.com/mobivoc/LithiumTitanate>
    <http://www.w3.org/2000/01/rdf-schema#comment> "A type of rechargeable battery, which has the advantage of being faster to charge than other lithium-ion batteries." ;
    <http://www.w3.org/2000/01/rdf-schema#label> "Lithium–titanate Battery"@en, "Lithium–titanate-Akkumulator"@de ;
    <http://www.w3.org/2000/01/rdf-schema#subClassOf> <http://eccenca.com/mobivoc/Battery> .

<http://eccenca.com/mobivoc/Longevity>
    a rdf:Property, <http://www.w3.org/2002/07/owl#DatatypeProperty> ;
    <http://www.w3.org/2000/01/rdf-schema#comment> "Indicates the period of time that a battery can still work ." ;
    <http://www.w3.org/2000/01/rdf-schema#domain> <http://eccenca.com/mobivoc/Battery> ;
    <http://www.w3.org/2000/01/rdf-schema#label> "Langlebigkeit"@de, "Longevity"@en ;
    <http://www.w3.org/2000/01/rdf-schema#range> <http://www.w3.org/2000/01/rdf-schema#Literal> .

<http://eccenca.com/mobivoc/MoltenSalt>
    <http://www.w3.org/2000/01/rdf-schema#comment> "A type of battery that uses molten salts as an electrolyte and offers both a high energy density and a high power density." ;
    <http://www.w3.org/2000/01/rdf-schema#label> "Molten salt Battery"@en, "Thermalbatterie"@de ;
    <http://www.w3.org/2000/01/rdf-schema#subClassOf> <http://eccenca.com/mobivoc/Battery> .

<http://eccenca.com/mobivoc/NickelCadmium>
    <http://www.w3.org/2000/01/rdf-schema#altlabel> "NiCd"@en, "NiCd-Akku"@de ;
    <http://www.w3.org/2000/01/rdf-schema#comment> "A type of rechargeable battery using nickel oxide hydroxide and metallic cadmium as electrodes." ;
    <http://www.w3.org/2000/01/rdf-schema#label> "Nickel-Cadmium-Akkumulator"@de, "Nickel–cadmium battery"@en ;
    <http://www.w3.org/2000/01/rdf-schema#subClassOf> <http://eccenca.com/mobivoc/Battery> ;
    <http://www.w3.org/2004/02/skos/core#hiddenLabel> "NiCad"@en .

<http://eccenca.com/mobivoc/NickelMetalHydride>
    <http://www.w3.org/2000/01/rdf-schema#altlabel> "NiMH"@de, "NiMH"@en ;
    <http://www.w3.org/2000/01/rdf-schema#comment> "A type of rechargeable battery. The chemical reaction at the positive electrode (cathode) is similar to that of the nickel–cadmium cell." ;
    <http://www.w3.org/2000/01/rdf-schema#label> "Nickel-Metallhydrid-Akkumulator"@de, "Nickel–metal hydride battery"@en ;
    <http://www.w3.org/2000/01/rdf-schema#subClassOf> <http://eccenca.com/mobivoc/Battery> ;
    <http://www.w3.org/2004/02/skos/core#hiddenLabel> "Ni–MH"@en .

<http://eccenca.com/mobivoc/NickelZinc>
    <http://www.w3.org/2000/01/rdf-schema#altlabel> "NiZn"@en ;
    <http://www.w3.org/2000/01/rdf-schema#comment> "A type of rechargeable battery which uses a stabilized zinc electrode system." ;
    <http://www.w3.org/2000/01/rdf-schema#label> "Nickel-Zinc Battery"@en, "Nickel-Zink-Akkumulator"@de ;
    <http://www.w3.org/2000/01/rdf-schema#subClassOf> <http://eccenca.com/mobivoc/Battery> .

<http://eccenca.com/mobivoc/Performance>
    a rdf:Property, <http://www.w3.org/2002/07/owl#DatatypeProperty> ;
    <http://www.w3.org/2000/01/rdf-schema#comment> "It reflects the condition of the battery when driving the EV in blistering summer heat and freezing temperatures." ;
    <http://www.w3.org/2000/01/rdf-schema#domain> <http://eccenca.com/mobivoc/Battery> ;
    <http://www.w3.org/2000/01/rdf-schema#label> "Leistung"@de, "Performance"@en ;
    <http://www.w3.org/2000/01/rdf-schema#range> <http://www.w3.org/2000/01/rdf-schema#Literal> .

<http://eccenca.com/mobivoc/Price>
    a rdf:Property, <http://www.w3.org/2002/07/owl#DatatypeProperty> ;
    <http://www.w3.org/2000/01/rdf-schema#comment> "Indicates the price of the battery." ;
    <http://www.w3.org/2000/01/rdf-schema#domain> <http://eccenca.com/mobivoc/Battery> ;
    <http://www.w3.org/2000/01/rdf-schema#label> "Preis"@de, "Price"@en ;
    <http://www.w3.org/2000/01/rdf-schema#range> <http://www.w3.org/2000/01/rdf-schema#Literal> .

<http://eccenca.com/mobivoc/ValveRegulatedLeadAcid>
    <http://www.w3.org/2000/01/rdf-schema#altlabel> "sealed battery"@en ;
    <http://www.w3.org/2000/01/rdf-schema#comment> "Α type of lead-acid rechargeable battery" ;
    <http://www.w3.org/2000/01/rdf-schema#label> "VRLA-Akkumulator"@de, "Valve-regulated lead-acid battery"@en ;
    <http://www.w3.org/2000/01/rdf-schema#subClassOf> <http://eccenca.com/mobivoc/LeadAcid> ;
    <http://www.w3.org/2004/02/skos/core#hiddenLabel> "VRLA "@en .

<http://eccenca.com/mobivoc/Watt>
    a rdf:Property, <http://www.w3.org/2002/07/owl#DatatypeProperty> ;
    <http://www.w3.org/2000/01/rdf-schema#comment> "Expresses the rate of energy conversion or transfer with respect to time." ;
    <http://www.w3.org/2000/01/rdf-schema#domain> <http://eccenca.com/mobivoc/Battery> ;
    <http://www.w3.org/2000/01/rdf-schema#label> "Watt"@de, "Watt"@en ;
    <http://www.w3.org/2000/01/rdf-schema#range> <http://www.w3.org/2000/01/rdf-schema#Literal> .

<http://eccenca.com/mobivoc/ZincAir>
    <http://www.w3.org/2000/01/rdf-schema#comment> "A metal-air battery powered by oxidizing zinc with oxygen from the air. These batteries have high energy densities and are relatively inexpensive to produce." ;
    <http://www.w3.org/2000/01/rdf-schema#label> "Zinc–air battery"@en, "Zink-Luft-Batterie"@de ;
    <http://www.w3.org/2000/01/rdf-schema#subClassOf> <http://eccenca.com/mobivoc/Battery> .

<http://eccenca.com/mobivoc/hasCRate>
    a rdf:Property, <http://www.w3.org/2002/07/owl#DatatypeProperty> ;
    <http://www.w3.org/2000/01/rdf-schema#comment> "The C-rate is a measure of the rate at which a battery is being discharged." ;
    <http://www.w3.org/2000/01/rdf-schema#domain> <http://eccenca.com/mobivoc/Battery> ;
    <http://www.w3.org/2000/01/rdf-schema#label> "CRate"@de, "CRate"@en ;
    <http://www.w3.org/2000/01/rdf-schema#range> <http://www.w3.org/2000/01/rdf-schema#Literal> .

<http://eccenca.com/mobivoc/hasCapacity>
    a rdf:Property, <http://www.w3.org/2002/07/owl#DatatypeProperty> ;
    <http://www.w3.org/2000/01/rdf-schema#comment> "It is the amount of electric charge it can deliver at the rated voltage. It is measured in units such as Ampere-hour (Ah), Watt-hour (Wh), kiloWatt-hour (kWh)." ;
    <http://www.w3.org/2000/01/rdf-schema#domain> <http://eccenca.com/mobivoc/Battery> ;
    <http://www.w3.org/2000/01/rdf-schema#label> "Capacity"@en, "Kapazität"@de ;
    <http://www.w3.org/2000/01/rdf-schema#range> <http://www.w3.org/2000/01/rdf-schema#Literal> .

<http://eccenca.com/mobivoc/hasCellVoltage>
    a rdf:Property, <http://www.w3.org/2002/07/owl#DatatypeProperty> ;
    <http://www.w3.org/2000/01/rdf-schema#altlabel> "Cell nominal Voltage"@en ;
    <http://www.w3.org/2000/01/rdf-schema#comment> "Represents either a source of energy or lost, used, or stored energy. It is measured in Voltage(V)." ;
    <http://www.w3.org/2000/01/rdf-schema#domain> <http://eccenca.com/mobivoc/Battery> ;
    <http://www.w3.org/2000/01/rdf-schema#label> "CellVoltage"@en, "Spannung"@de ;
    <http://www.w3.org/2000/01/rdf-schema#range> <http://www.w3.org/2000/01/rdf-schema#Literal> .

<http://eccenca.com/mobivoc/hasChargeTime>
    a rdf:Property, <http://www.w3.org/2002/07/owl#DatatypeProperty> ;
    <http://www.w3.org/2000/01/rdf-schema#comment> "Indicates the time that is needed for a battery's full charge." ;
    <http://www.w3.org/2000/01/rdf-schema#domain> <http://eccenca.com/mobivoc/Battery> ;
    <http://www.w3.org/2000/01/rdf-schema#label> "Charge time"@en, "Ladezeit"@de ;
    <http://www.w3.org/2000/01/rdf-schema#range> <http://www.w3.org/2000/01/rdf-schema#Literal> .

<http://eccenca.com/mobivoc/hasCycleLife>
    a rdf:Property, <http://www.w3.org/2002/07/owl#DatatypeProperty> ;
    <http://www.w3.org/2000/01/rdf-schema#comment> "The cycle life is the number of complete charge/discharge cycles that the battery is able to support before that its capacity falls under 80% of it's original capacity." ;
    <http://www.w3.org/2000/01/rdf-schema#domain> <http://eccenca.com/mobivoc/Battery> ;
    <http://www.w3.org/2000/01/rdf-schema#label> "Batterielebensdauer"@de, "Cycle Life"@en ;
    <http://www.w3.org/2000/01/rdf-schema#range> <http://www.w3.org/2000/01/rdf-schema#Literal> .

<http://eccenca.com/mobivoc/hasOperatingTemperature>
    a rdf:Property, <http://www.w3.org/2002/07/owl#DatatypeProperty> ;
    <http://www.w3.org/2000/01/rdf-schema#comment> "Battery operating temperature is the temperature at which a battery operates effectively." ;
    <http://www.w3.org/2000/01/rdf-schema#domain> <http://eccenca.com/mobivoc/Battery> ;
    <http://www.w3.org/2000/01/rdf-schema#label> "Betriebstemperatur"@de, "Operating temperature"@en ;
    <http://www.w3.org/2000/01/rdf-schema#range> <http://www.w3.org/2000/01/rdf-schema#Literal> .

<http://eccenca.com/mobivoc/hasSelfDischarge>
    a rdf:Property, <http://www.w3.org/2002/07/owl#DatatypeProperty> ;
    <http://www.w3.org/2000/01/rdf-schema#comment> "Self-discharge is the electrical capacity that is lost when the cell simply sits on the shelf. It is highly dependent on temperature, increasing as the battery temperature is increased." ;
    <http://www.w3.org/2000/01/rdf-schema#domain> <http://eccenca.com/mobivoc/Battery> ;
    <http://www.w3.org/2000/01/rdf-schema#label> "Selbstentladung"@de, "Self Discharge"@en ;
    <http://www.w3.org/2000/01/rdf-schema#range> <http://www.w3.org/2000/01/rdf-schema#Literal> .

<http://eccenca.com/mobivoc/hasSpecificEnergyDensity>
    a rdf:Property, <http://www.w3.org/2002/07/owl#DatatypeProperty> ;
    <http://www.w3.org/2000/01/rdf-schema#comment> "It is the amount of energy stored in a given system or region of space per unit volume or mass. It is measured in Wh/kg." ;
    <http://www.w3.org/2000/01/rdf-schema#domain> <http://eccenca.com/mobivoc/Battery> ;
    <http://www.w3.org/2000/01/rdf-schema#label> "Energiedichte"@de, "Specific Energy Density"@en ;
    <http://www.w3.org/2000/01/rdf-schema#range> <http://www.w3.org/2000/01/rdf-schema#Literal> .

<http://eccenca.com/mobivoc/hasSpecificPower>
    a rdf:Property, <http://www.w3.org/2002/07/owl#DatatypeProperty> ;
    <http://www.w3.org/2000/01/rdf-schema#comment> "Specific power demonstrates acceleration. It is the power that can be derived per unit weight of the cell (W/kg)." ;
    <http://www.w3.org/2000/01/rdf-schema#domain> <http://eccenca.com/mobivoc/Battery> ;
    <http://www.w3.org/2000/01/rdf-schema#label> " Leistungskonstante"@de, "Specific Power"@en ;
    <http://www.w3.org/2000/01/rdf-schema#range> <http://www.w3.org/2000/01/rdf-schema#Literal> .

<http://eccenca.com/mobivoc/petrolBatteryHybrid>
    <http://www.w3.org/2000/01/rdf-schema#comment> "****" ;
    <http://www.w3.org/2000/01/rdf-schema#label> "PetrolBatterieHybrid"@de, "PetrolBatteryHybrid"@en ;
    <http://www.w3.org/2000/01/rdf-schema#subClassOf> <http://eccenca.com/mobivoc/Battery> .

<http://purl.org/net/mobivoc/BicycleDockingStation>
    a <http://www.w3.org/2000/01/rdf-schema#Class>, <http://www.w3.org/2002/07/owl#Class> ;
    <http://www.w3.org/2000/01/rdf-schema#comment> "A docking station of a bicycle sharing system for picking up and returning bicycles." ;
    <http://www.w3.org/2000/01/rdf-schema#label> "Fahrradstation"@de, "bicycle docking station"@en, "test"@em, "test"@es, "test2"@me, "testmodify"@em .

<http://purl.org/net/mobivoc/dockingStationNumber>
    a rdf:Property, <http://www.w3.org/2002/07/owl#DatatypeProperty> ;
    <http://www.w3.org/2000/01/rdf-schema#comment> "Identification number of the bicycle docking station." ;
    <http://www.w3.org/2000/01/rdf-schema#domain> <http://purl.org/net/mobivoc/BicycleDockingStation> ;
    <http://www.w3.org/2000/01/rdf-schema#label> "Stationsnummer"@de, "docking station number"@en ;
    <http://www.w3.org/2000/01/rdf-schema#range> <http://www.w3.org/2000/01/rdf-schema#Literal> .

<http://purl.org/net/mobivoc/numberOfBicyclesAvailable>
    a rdf:Property, <http://www.w3.org/2002/07/owl#DatatypeProperty> ;
    <http://www.w3.org/2000/01/rdf-schema#comment> "Indicates the number of bicycles available at the docking station." ;
    <http://www.w3.org/2000/01/rdf-schema#domain> <http://purl.org/net/mobivoc/BicycleDockingStation> ;
    <http://www.w3.org/2000/01/rdf-schema#label> "Anzahl verfügbarer Fahrräder"@de, "number of bicycles available"@en ;
    <http://www.w3.org/2000/01/rdf-schema#range> <http://www.w3.org/2000/01/rdf-schema#Literal> .

<http://purl.org/net/mobivoc/numberOfDockingPoints>
    a rdf:Property, <http://www.w3.org/2002/07/owl#DatatypeProperty> ;
    <http://www.w3.org/2000/01/rdf-schema#comment> "Indicates the number of docking points for bicycles." ;
    <http://www.w3.org/2000/01/rdf-schema#domain> <http://purl.org/net/mobivoc/BicycleDockingStation> ;
    <http://www.w3.org/2000/01/rdf-schema#label> "Anzahl Fahrradstellplätze"@de, "number of docking points"@en ;
    <http://www.w3.org/2000/01/rdf-schema#range> <http://www.w3.org/2000/01/rdf-schema#Literal> .

<http://purl.org/net/mobivoc/numberOfSpacesAvailable>
    a rdf:Property, <http://www.w3.org/2002/07/owl#DatatypeProperty> ;
    <http://www.w3.org/2000/01/rdf-schema#comment> "Indicates the number of spaces available at the docking station." ;
    <http://www.w3.org/2000/01/rdf-schema#domain> <http://purl.org/net/mobivoc/BicycleDockingStation> ;
    <http://www.w3.org/2000/01/rdf-schema#label> "Anzahl freier Stellplätze"@de, "number of spaces available"@en ;
    <http://www.w3.org/2000/01/rdf-schema#range> <http://www.w3.org/2000/01/rdf-schema#Literal> .

